doc/developer/semantics/Mz.lean
@@ -16,3 +16,4 @@ import Mz.Collection
 import Mz.Schema
 import Mz.OutputType
 import Mz.Legal
+import Mz.WellTyped
